code/k256/Hacl.Spec.K256.Field52.Lemmas3.fst
@@ -1,0 +1,696 @@
+module Hacl.Spec.K256.Field52.Lemmas3
+
+open FStar.Mul
+open Lib.IntTypes
+
+module S = Spec.K256
+
+include Hacl.Spec.K256.Field52.Definitions
+include Hacl.Spec.K256.Field52
+
+module LD = Hacl.Spec.K256.Field52.Definitions.Lemmas
+module L4 = Hacl.Spec.K256.Field52.Lemmas4
+
+
+#set-options "--z3rlimit 100 --fuel 0 --ifuel 0"
+
+
+val lemma_bound_mul64_wide (ma mb:nat) (mma mmb:nat) (a b:uint64) : Lemma
+  (requires v a <= ma * mma /\ v b <= mb * mmb)
+  (ensures  (let r = mul64_wide a b in
+    v r = v a * v b /\ v r <= ma * mb * (mma * mmb)))
+
+let lemma_bound_mul64_wide ma mb mma mmb a b =
+  let r = mul64_wide a b in
+  assert (v r = v a * v b);
+  calc (<=) {
+    v a * v b;
+    (<=) { Math.Lemmas.lemma_mult_le_right (v b) (v a) (ma * mma) }
+    (ma * mma) * v b;
+    (<=) { Math.Lemmas.lemma_mult_le_left (ma * mma) (v b) (mb * mmb) }
+    (ma * mma) * (mb * mmb);
+    (==) { Math.Lemmas.paren_mul_right ma mma (mb * mmb) }
+    ma * (mma * (mb * mmb));
+    (==) {
+      Math.Lemmas.paren_mul_right mma mb mmb;
+      Math.Lemmas.swap_mul mma mb;
+      Math.Lemmas.paren_mul_right mb mma mmb }
+    ma * (mb * (mma * mmb));
+    (==) { Math.Lemmas.paren_mul_right ma mb (mma * mmb) }
+    ma * mb * (mma * mmb);
+  }
+
+
+val lemma_four_mul64_wide (a0 a1 a2 a3 b0 b1 b2 b3:uint64) : Lemma
+  (requires
+    felem_fits1 a0 8 /\ felem_fits1 b0 8 /\
+    felem_fits1 a1 8 /\ felem_fits1 b1 8 /\
+    felem_fits1 a2 8 /\ felem_fits1 b2 8 /\
+    felem_fits1 a3 8 /\ felem_fits1 b3 8)
+  (ensures
+   (let d = mul64_wide a0 b3 +. mul64_wide a1 b2 +. mul64_wide a2 b1 +. mul64_wide a3 b0 in
+    v d = v a0 * v b3 + v a1 * v b2 + v a2 * v b1 + v a3 * v b0 /\
+    v d <= 256 * (max52 * max52)))
+
+let lemma_four_mul64_wide a0 a1 a2 a3 b0 b1 b2 b3 =
+  lemma_bound_mul64_wide 8 8 max52 max52 a0 b3;
+  lemma_bound_mul64_wide 8 8 max52 max52 a1 b2;
+  lemma_bound_mul64_wide 8 8 max52 max52 a2 b1;
+  lemma_bound_mul64_wide 8 8 max52 max52 a3 b0;
+  assert (v a0 * v b3 + v a1 * v b2 + v a2 * v b1 + v a3 * v b0 <= 256 * (max52 * max52));
+  assert_norm (256 * (max52 * max52) < pow2 128);
+
+  Math.Lemmas.small_mod (v a0 * v b3 + v a1 * v b2) (pow2 128);
+  Math.Lemmas.small_mod (v a0 * v b3 + v a1 * v b2 + v a2 * v b1) (pow2 128);
+  Math.Lemmas.small_mod (v a0 * v b3 + v a1 * v b2 + v a2 * v b1 + v a3 * v b0) (pow2 128)
+
+
+val lemma_128_max52_max48: unit -> Lemma (128 * (max52 * max48) < 8 * (max52 * max52))
+let lemma_128_max52_max48 () =
+  assert_norm (128 * (max52 * max48) < 8 * (max52 * max52))
+
+
+val lemma_add_five_mul64_wide (md:nat) (d:uint128) (a0 a1 a2 a3 a4 b0 b1 b2 b3 b4:uint64) : Lemma
+  (requires
+    v d <= md * max52 /\ md <= 321 /\
+    felem_fits1 a0 8 /\ felem_fits1 b0 8 /\
+    felem_fits1 a1 8 /\ felem_fits1 b1 8 /\
+    felem_fits1 a2 8 /\ felem_fits1 b2 8 /\
+    felem_fits1 a3 8 /\ felem_fits1 b3 8 /\
+    felem_fits_last1 a4 8 /\ felem_fits_last1 b4 8)
+  (ensures
+   (let d1 = d +. mul64_wide a0 b4 +. mul64_wide a1 b3 +.
+     mul64_wide a2 b2 +. mul64_wide a3 b1 +. mul64_wide a4 b0 in
+    v d1 == v d + v a0 * v b4 + v a1 * v b3 + v a2 * v b2 + v a3 * v b1 + v a4 * v b0 /\
+    v d1 <= 201 * (max52 * max52)))
+
+let lemma_add_five_mul64_wide md d a0 a1 a2 a3 a4 b0 b1 b2 b3 b4 =
+  lemma_bound_mul64_wide 8 8 max52 max48 a0 b4;
+  lemma_bound_mul64_wide 8 8 max52 max52 a1 b3;
+  lemma_bound_mul64_wide 8 8 max52 max52 a2 b2;
+  lemma_bound_mul64_wide 8 8 max52 max52 a3 b1;
+  lemma_bound_mul64_wide 8 8 max48 max52 a4 b0;
+  Math.Lemmas.swap_mul max52 max48;
+  assert (v d + v a0 * v b4 + v a1 * v b3 + v a2 * v b2 + v a3 * v b1 + v a4 * v b0 <=
+    md * max52 + 128 * (max52 * max48) + 192 * (max52 * max52));
+  lemma_128_max52_max48 ();
+  assert_norm (md * max52 + 128 * (max52 * max48) + 192 * (max52 * max52) <= 201 * (max52 * max52));
+  assert_norm (201 * (max52 * max52) < pow2 128);
+
+  Math.Lemmas.small_mod (v d + v a0 * v b4) (pow2 128);
+  Math.Lemmas.small_mod (v d + v a0 * v b4 + v a1 * v b3) (pow2 128);
+  Math.Lemmas.small_mod (v d + v a0 * v b4 + v a1 * v b3 + v a2 * v b2) (pow2 128);
+  Math.Lemmas.small_mod (v d + v a0 * v b4 + v a1 * v b3 + v a2 * v b2 + v a3 * v b1) (pow2 128);
+  Math.Lemmas.small_mod (v d + v a0 * v b4 + v a1 * v b3 + v a2 * v b2 + v a3 * v b1 + v a4 * v b0) (pow2 128)
+
+
+val lemma_add_four_mul64_wide (md:nat) (d:uint128) (a1 a2 a3 a4 b1 b2 b3 b4:uint64) : Lemma
+  (requires
+    v d <= md * max52 /\ md <= 321 /\
+    felem_fits1 a1 8 /\ felem_fits1 b1 8 /\
+    felem_fits1 a2 8 /\ felem_fits1 b2 8 /\
+    felem_fits1 a3 8 /\ felem_fits1 b3 8 /\
+    felem_fits_last1 a4 8 /\ felem_fits_last1 b4 8)
+  (ensures
+   (let d1 = d +. mul64_wide a1 b4 +. mul64_wide a2 b3 +.
+     mul64_wide a3 b2 +. mul64_wide a4 b1 in
+    v d1 == v d + v a1 * v b4 + v a2 * v b3 + v a3 * v b2 + v a4 * v b1 /\
+    v d1 <= 201 * (max52 * max52)))
+
+let lemma_add_four_mul64_wide md d a1 a2 a3 a4 b1 b2 b3 b4 =
+  Math.Lemmas.small_mod (v (d +. mul64_wide a1 b4 +. mul64_wide a2 b3
+       +. mul64_wide a3 b2 +. mul64_wide a4 b1)) (pow2 128);
+  assert_norm (max48 < max52);
+  lemma_add_five_mul64_wide 321 d a1 a2 a3 a4 (u64 0) (u64 0) b1 b2 b3 b4
+
+
+val lemma_add_three_mul64_wide52 (md:nat) (d:uint128) (a0 a1 a2 b0 b1 b2:uint64) : Lemma
+  (requires
+    v d <= md * max52 /\ md <= 130 /\
+    felem_fits1 a0 8 /\ felem_fits1 b0 8 /\
+    felem_fits1 a1 8 /\ felem_fits1 b1 8 /\
+    felem_fits1 a2 8 /\ felem_fits1 b2 8)
+  (ensures
+   (let d1 = d +. mul64_wide a0 b2 +. mul64_wide a1 b1 +. mul64_wide a2 b0 in
+    v d1 == v d + v a0 * v b2 + v a1 * v b1 + v a2 * v b0 /\
+    v d1 <= 193 * (max52 * max52)))
+
+let lemma_add_three_mul64_wide52 md d a0 a1 a2 b0 b1 b2 =
+  lemma_bound_mul64_wide 8 8 max52 max52 a0 b2;
+  lemma_bound_mul64_wide 8 8 max52 max52 a1 b1;
+  lemma_bound_mul64_wide 8 8 max52 max52 a2 b0;
+  assert (v d + v a0 * v b2 + v a1 * v b1 + v a2 * v b0 <= md * max52 + 192 * (max52 * max52));
+  assert_norm (md * max52 + 192 * (max52 * max52) <= 193 * (max52 * max52));
+  assert_norm (193 * (max52 * max52) < pow2 128);
+
+  Math.Lemmas.small_mod (v d + v a0 * v b2) (pow2 128);
+  Math.Lemmas.small_mod (v d + v a0 * v b2 + v a1 * v b1) (pow2 128);
+  Math.Lemmas.small_mod (v d + v a0 * v b2 + v a1 * v b1 + v a2 * v b0) (pow2 128)
+
+
+val lemma_add_three_mul64_wide (md:nat) (d:uint128) (a2 a3 a4 b2 b3 b4:uint64) : Lemma
+  (requires
+    v d <= md * max52 /\ md <= 320 /\
+    felem_fits1 a2 8 /\ felem_fits1 b2 8 /\
+    felem_fits1 a3 8 /\ felem_fits1 b3 8 /\
+    felem_fits_last1 a4 8 /\ felem_fits_last1 b4 8)
+  (ensures
+   (let d1 = d +. mul64_wide a2 b4 +. mul64_wide a3 b3 +. mul64_wide a4 b2 in
+    v d1 == v d + v a2 * v b4 + v a3 * v b3 + v a4 * v b2 /\
+    v d1 <= 73 * (max52 * max52)))
+
+let lemma_add_three_mul64_wide md d a2 a3 a4 b2 b3 b4 =
+  lemma_bound_mul64_wide 8 8 max52 max48 a2 b4;
+  lemma_bound_mul64_wide 8 8 max52 max52 a3 b3;
+  lemma_bound_mul64_wide 8 8 max48 max52 a4 b2;
+
+  Math.Lemmas.swap_mul max52 max48;
+  assert (v d + v a2 * v b4 + v a3 * v b3 + v a4 * v b2 <=
+    md * max52 + 128 * (max52 * max48) + 64 * (max52 * max52));
+  lemma_128_max52_max48 ();
+  assert_norm (md * max52 + 128 * (max52 * max48) + 64 * (max52 * max52) <= 73 * (max52 * max52));
+  assert_norm (73 * (max52 * max52) < pow2 128);
+
+  Math.Lemmas.small_mod (v d + v a2 * v b4) (pow2 128);
+  Math.Lemmas.small_mod (v d + v a2 * v b4 + v a3 * v b3) (pow2 128);
+  Math.Lemmas.small_mod (v d + v a2 * v b4 + v a3 * v b3 + v a4 * v b2) (pow2 128)
+
+
+val lemma_add_two_mul64_wide52 (md:nat) (d:uint128) (a0 a1 b0 b1:uint64) : Lemma
+  (requires
+    v d <= md * max52 /\ md <= 129 /\
+    felem_fits1 a0 8 /\ felem_fits1 b0 8 /\
+    felem_fits1 a1 8 /\ felem_fits1 b1 8)
+  (ensures
+   (let d1 = d +. mul64_wide a0 b1 +. mul64_wide a1 b0 in
+    v d1 == v d + v a0 * v b1 + v a1 * v b0 /\
+    v d1 <= 129 * (max52 * max52)))
+
+let lemma_add_two_mul64_wide52 md d a0 a1 b0 b1 =
+  lemma_bound_mul64_wide 8 8 max52 max52 a0 b1;
+  lemma_bound_mul64_wide 8 8 max52 max52 a1 b0;
+  assert (v d + v a0 * v b1 + v a1 * v b0 <= md * max52 + 128 * (max52 * max52));
+  assert_norm (md * max52 + 128 * (max52 * max52) <= 129 * (max52 * max52));
+  assert_norm (md * max52 + 128 * (max52 * max52) < pow2 128);
+  Math.Lemmas.small_mod (v d + v a0 * v b1) (pow2 128);
+  Math.Lemmas.small_mod (v d + v a0 * v b1 + v a1 * v b0) (pow2 128)
+
+
+val lemma_add_two_mul64_wide (md:nat) (d:uint128) (a3 a4 b3 b4:uint64) : Lemma
+  (requires
+    v d <= md * max52 /\ md <= 129 /\
+    felem_fits1 a3 8 /\ felem_fits1 b3 8 /\
+    felem_fits_last1 a4 8 /\ felem_fits_last1 b4 8)
+  (ensures
+   (let d1 = d +. mul64_wide a3 b4 +. mul64_wide a4 b3 in
+    v d1 == v d + v a3 * v b4 + v a4 * v b3 /\
+    v d1 <= 9 * (max52 * max52)))
+
+let lemma_add_two_mul64_wide md d a3 a4 b3 b4 =
+  lemma_bound_mul64_wide 8 8 max52 max48 a3 b4;
+  lemma_bound_mul64_wide 8 8 max48 max52 a4 b3;
+  Math.Lemmas.swap_mul max52 max48;
+  assert (v d + v a3 * v b4 + v a4 * v b3 <= md * max52 + 128 * (max52 * max48));
+  lemma_128_max52_max48 ();
+  assert_norm (md * max52 + 128 * (max52 * max48) <= 9 * (max52 * max52));
+  assert_norm (9 * (max52 * max52) < pow2 128);
+  Math.Lemmas.small_mod (v d + v a3 * v b4) (pow2 128);
+  Math.Lemmas.small_mod (v d + v a3 * v b4 + v a4 * v b3) (pow2 128)
+
+
+val lemma_r_lsh12: unit ->
+  Lemma (let rs = u64 0x1000003D10 <<. 12ul in
+    v rs = 0x1000003D10 * pow2 12 /\ v rs < pow2 49)
+
+let lemma_r_lsh12 () =
+  let rs = u64 0x1000003D10 <<. 12ul in
+  assert_norm (0x1000003D10 < pow2 37);
+  assert (v rs = 0x1000003D10 * pow2 12 % pow2 64);
+  Math.Lemmas.lemma_mult_le_right (pow2 12) 0x1000003D10 (pow2 37);
+  Math.Lemmas.pow2_plus 12 37;
+  assert (0x1000003D10 * pow2 12 < pow2 49);
+  Math.Lemmas.pow2_lt_compat 64 49;
+  Math.Lemmas.small_mod (0x1000003D10 * pow2 12) (pow2 64);
+  assert (v rs = 0x1000003D10 * pow2 12)
+
+
+val lemma_r_rsh4: unit ->
+  Lemma (let rs = u64 0x1000003D10 >>. 4ul in
+    v rs = 0x1000003D10 / pow2 4 /\ v rs < pow2 33)
+
+let lemma_r_rsh4 () =
+  let rs = u64 0x1000003D10 >>. 4ul in
+  assert_norm (0x1000003D10 < pow2 37);
+  Math.Lemmas.lemma_div_lt 0x1000003D10 37 4
+
+
+val lemma_add_mul64_wide (pa pb md:nat) (d:uint128) (a b:uint64) : Lemma
+  (requires
+    v a < pow2 pa /\ v b < pow2 pb /\ md + 1 <= 500 /\ // md + 1 <= pow2 24
+    v d <= md * (max52 * max52) /\ pa + pb <= 103)
+  (ensures (let r = d +. mul64_wide a b in
+    v r = v d + v a * v b /\ v r <= (md + 1) * (max52 * max52)))
+
+let lemma_add_mul64_wide pa pb md d a b =
+  let r = d +. mul64_wide a b in
+  lemma_bound_mul64_wide 1 1 (pow2 pa) (pow2 pb) a b;
+  assert (v d + v a * v b <= md * (max52 * max52) + pow2 pa * pow2 pb);
+  Math.Lemmas.pow2_plus pa pb;
+  Math.Lemmas.pow2_le_compat 103 (pa + pb);
+  assert_norm (pow2 103 < max52 * max52);
+  assert (v d + v a * v b <= md * (max52 * max52) + max52 * max52);
+  Math.Lemmas.lemma_mult_le_right (max52 * max52) (md + 1) 500;
+  assert_norm (500 * (max52 * max52) < pow2 128);
+  Math.Lemmas.small_mod (v d + v a * v b) (pow2 128)
+
+
+val lemma_bound_add_mul64_wide_r (md:nat) (d c:uint128) : Lemma
+  (requires v d <= md * (max52 * max52) /\ md <= 256)
+  (ensures  (let r = d +. mul64_wide (u64 0x1000003D10) (to_u64 c) in
+    v r = v d + 0x1000003D10 * (v c % pow2 64) /\ v r <= (md + 1) * (max52 * max52)))
+
+let lemma_bound_add_mul64_wide_r md d c =
+  assert_norm (0x1000003D10 < pow2 37);
+  lemma_add_mul64_wide 37 64 md d (u64 0x1000003D10) (to_u64 c)
+
+
+val lemma_bound_add_mul64_wide_r_lsh12 (md:nat) (d:uint128) (c:uint64) : Lemma
+  (requires v d <= md * (max52 * max52) /\ md <= 320 /\ v c <= pow2 38)
+  (ensures  (let r = d +. mul64_wide (u64 0x1000003D10 <<. 12ul) c in
+    v r = v d + 0x1000003D10 * pow2 12 * v c /\ v r <= (md + 1) * (max52 * max52)))
+
+let lemma_bound_add_mul64_wide_r_lsh12 md d c =
+  let rs = u64 0x1000003D10 <<. 12ul in
+  lemma_r_lsh12 ();
+  Math.Lemmas.pow2_lt_compat 39 38;
+  lemma_add_mul64_wide 49 39 md d rs c
+
+
+val lemma_bound_add_mul64_wide_r_rsh4 (md:nat) (d:uint128) (c:uint64) : Lemma
+  (requires v d <= md * (max52 * max52) /\ md <= 64 /\ v c < pow2 56)
+  (ensures  (let r = d +. mul64_wide c (u64 0x1000003D10 >>. 4ul) in
+    v r = v d + v c * (0x1000003D10 / pow2 4) /\ v r <= (md + 1) * (max52 * max52)))
+
+let lemma_bound_add_mul64_wide_r_rsh4 md d c =
+  let rs = u64 0x1000003D10 >>. 4ul in
+  lemma_r_rsh4 ();
+  lemma_add_mul64_wide 33 56 md d rs c
+
+
+val lemma_bound_add_mul64_wide_r_lsh12_add (md:nat) (c:uint128) (d t3:uint64) : Lemma
+  (requires v c <= md * max52 /\ md <= 194 /\ v d < pow2 44 /\ felem_fits1 t3 1)
+  (ensures  (let r = c +. mul64_wide (u64 0x1000003D10 <<. 12ul) d +. to_u128 t3 in
+    v r = v c + 0x1000003D10 * pow2 12 * v d + v t3 /\ v r < pow2 94))
+
+let lemma_bound_add_mul64_wide_r_lsh12_add md c d t3 =
+  let rs = u64 0x1000003D10 <<. 12ul in
+  lemma_r_lsh12 ();
+
+  let r = c +. mul64_wide rs d in
+  lemma_bound_mul64_wide 1 1 (pow2 49) (pow2 44) rs d;
+  assert (v c + v rs * v d + v t3 < md * max52 + pow2 49 * pow2 44 + max52);
+  Math.Lemmas.pow2_plus 49 44;
+  assert (v c + v rs * v d + v t3 < md * max52 + pow2 93 + max52);
+  Math.Lemmas.distributivity_add_left md 1 max52;
+  assert (v c + v rs * v d + v t3 < (md + 1) * max52 + pow2 93);
+  Math.Lemmas.lemma_mult_le_right max52 (md + 1) 195;
+  assert_norm (195 * max52 < pow2 93);
+  Math.Lemmas.pow2_double_sum 93;
+  assert (195 * max52 + pow2 93 < pow2 94);
+  Math.Lemmas.pow2_lt_compat 128 94;
+  Math.Lemmas.small_mod (v c + v rs * v d + v t3) (pow2 128)
+
+
+val lemma_u128_div52: md:pos -> a:uint128 -> Lemma
+  (requires v a <= md * max52 * max52)
+  (ensures  v a / pow2 52 <= md * max52)
+
+let lemma_u128_div52 md a =
+  Math.Lemmas.lemma_mult_lt_left (md * max52) max52 (pow2 52);
+  Math.Lemmas.lemma_div_le (v a) (md * max52 * pow2 52) (pow2 52);
+  Math.Lemmas.multiple_division_lemma (md * max52) (pow2 52)
+
+
+val lemma_u128_div64_max48: md:pos -> a:uint128 -> Lemma
+  (requires v a <= md * (max48 * max48))
+  (ensures  v a / pow2 64 <= md * pow2 32)
+
+let lemma_u128_div64_max48 md a =
+  assert_norm (max48 < pow2 48);
+  Math.Lemmas.lemma_mult_le_left max48 max48 (pow2 48);
+  Math.Lemmas.lemma_mult_le_right (pow2 48) max48 (pow2 48);
+  Math.Lemmas.pow2_plus 48 48;
+  assert (max48 * max48 < pow2 96);
+  Math.Lemmas.lemma_mult_le_left md (max48 * max48) (pow2 96);
+  assert (v a < md * pow2 96);
+  Math.Lemmas.lemma_div_le (v a) (md * pow2 96) (pow2 64);
+  Math.Lemmas.pow2_plus 64 32;
+  Math.Lemmas.multiple_division_lemma (md * pow2 32) (pow2 64)
+
+
+val lemma_u128_div64_max52: md:pos -> a:uint128 -> Lemma
+  (requires v a <= md * (max52 * max52))
+  (ensures  v a / pow2 64 <= md * pow2 40)
+
+let lemma_u128_div64_max52 md a =
+  assert_norm (max52 < pow2 52);
+  Math.Lemmas.lemma_mult_le_left max52 max52 (pow2 52);
+  Math.Lemmas.lemma_mult_le_right (pow2 52) max52 (pow2 52);
+  Math.Lemmas.pow2_plus 52 52;
+  assert (max52 * max52 < pow2 104);
+  Math.Lemmas.lemma_mult_le_left md (max52 * max52) (pow2 104);
+  assert (v a < md * pow2 104);
+  Math.Lemmas.lemma_div_le (v a) (md * pow2 104) (pow2 64);
+  Math.Lemmas.pow2_plus 64 40;
+  Math.Lemmas.multiple_division_lemma (md * pow2 40) (pow2 64)
+
+
+val lemma_bound_c0: c0:uint128 -> Lemma
+  (requires v c0 <= 64 * (max48 * max48))
+  (ensures  v c0 / pow2 64 <= pow2 38)
+
+let lemma_bound_c0 c0 =
+  lemma_u128_div64_max48 64 c0;
+  assert_norm (pow2 6 = 64);
+  Math.Lemmas.pow2_plus 6 32
+
+
+val lemma_bound_d10: d10:uint128 -> Lemma
+  (requires v d10 <= 9 * (max52 * max52))
+  (ensures  v d10 / pow2 64 < pow2 44)
+
+let lemma_bound_d10 d10 =
+  lemma_u128_div64_max52 9 d10;
+  assert_norm (9 < pow2 4);
+  Math.Lemmas.lemma_mult_le_right (pow2 38) 9 (pow2 4);
+  Math.Lemmas.pow2_plus 4 40
+
+
+val lemma_bound_rsh64_to: a:uint128 ->
+  Lemma (v (to_u64 (a >>. 64ul)) = v a / pow2 64)
+
+let lemma_bound_rsh64_to a =
+  let r = to_u64 (a >>. 64ul) in
+  assert (v r == (v a / pow2 64) % pow2 64);
+  Math.Lemmas.lemma_div_lt (v a) 128 64;
+  Math.Lemmas.small_mod (v a / pow2 64) (pow2 64)
+
+
+val lemma_u128_to_u64_mask52: d:uint128 ->
+  Lemma (let r = to_u64 d &. mask52 in
+    v r = v d % pow2 52 /\ felem_fits1 r 1)
+
+let lemma_u128_to_u64_mask52 d =
+  let r = to_u64 d &. mask52 in
+  LD.lemma_mask52 (to_u64 d);
+  assert (v r = v d % pow2 64 % pow2 52);
+  Math.Lemmas.pow2_modulo_modulo_lemma_1 (v d) 52 64
+
+
+val lemma_bound_mask52_rsh52: md:pos -> d:uint128 -> Lemma
+  (requires v d <= md * (max52 * max52) /\ md <= 321)
+  (ensures (let r = to_u64 d &. mask52 in let k = d >>. 52ul in
+    v r = v d % pow2 52 /\ v k = v d / pow2 52 /\
+    felem_fits1 r 1 /\ v k <= md * max52))
+
+let lemma_bound_mask52_rsh52 md d =
+  lemma_u128_to_u64_mask52 d;
+  lemma_u128_div52 md d
+
+
+val lemma_bound_add_mul64_wide_r_mask52 (md:pos) (d8 c5:uint128) : Lemma
+  (requires v d8 <= md * (max52 * max52) /\ v c5 <= md * (max52 * max52) /\ md <= 129)
+  (ensures  (let r = c5 +. mul64_wide (to_u64 d8 &. mask52) (u64 0x1000003D10) in
+    let d9 = d8 >>. 52ul in v d9 = v d8 / pow2 52 /\ v d9 <= md * max52 /\
+    v r = v c5 + v d8 % pow2 52 * 0x1000003D10 /\ v r <= (md + 1) * (max52 * max52)))
+
+let lemma_bound_add_mul64_wide_r_mask52 md d8 c5 =
+  let tm = to_u64 d8 &. mask52 in
+  lemma_bound_mask52_rsh52 md d8;
+  assert_norm (0x1000003D10 < pow2 37);
+  lemma_add_mul64_wide 64 37 md c5 tm (u64 0x1000003D10)
+
+
+val lemma_bound_mask48_rsh48: t4:uint64 -> Lemma
+  (requires felem_fits1 t4 1)
+  (ensures (let tx = t4 >>. 48ul in let r = t4 &. mask48 in
+    v tx = v t4 / pow2 48 /\ v r = v t4 % pow2 48 /\
+    felem_fits_last1 r 1 /\ v tx < pow2 4))
+
+let lemma_bound_mask48_rsh48 t4 =
+  LD.lemma_mask48 t4;
+  Math.Lemmas.lemma_div_lt (v t4) 52 48
+
+
+val lemma_bound_mask52_rsh52_sp: d:uint128 -> Lemma
+  (requires v d < pow2 94)
+  (ensures (let r = to_u64 d &. mask52 in let k = to_u64 (d >>. 52ul) in
+    v r = v d % pow2 52 /\ v k = v d / pow2 52 /\
+    felem_fits1 r 1 /\ v k < pow2 42))
+
+let lemma_bound_mask52_rsh52_sp d =
+  let r = to_u64 d &. mask52 in
+  lemma_u128_to_u64_mask52 d;
+
+  let k = to_u64 (d >>. 52ul) in
+  assert (v k == v d / pow2 52 % pow2 64);
+  Math.Lemmas.lemma_div_lt (v d) 94 52;
+  Math.Lemmas.pow2_lt_compat 64 42;
+  Math.Lemmas.small_mod (v d / pow2 52) (pow2 64)
+
+
+val lemma_tx_logor_u0_lsh4 (tx u0:uint64) : Lemma
+  (requires v tx < pow2 4 /\ felem_fits1 u0 1)
+  (ensures (let u0' = tx |. (u0 <<. 4ul) in
+    v u0' == v tx + v u0 * pow2 4 /\ v u0' < pow2 56))
+
+let lemma_tx_logor_u0_lsh4 tx u0 =
+  let u0' = tx |. (u0 <<. 4ul) in
+  assert (v (u0 <<. 4ul) = v u0 * pow2 4 % pow2 64);
+  Math.Lemmas.lemma_mult_le_right (pow2 4) (v u0) (pow2 52 - 1);
+  Math.Lemmas.distributivity_sub_left (pow2 52) 1 (pow2 4);
+  Math.Lemmas.pow2_plus 52 4;
+  assert (v u0 * pow2 4 <= pow2 56 - pow2 4);
+  Math.Lemmas.pow2_lt_compat 64 56;
+  Math.Lemmas.small_mod (v u0 * pow2 4) (pow2 64);
+  assert (v (u0 <<. 4ul) = v u0 * pow2 4 % pow2 64);
+
+  Math.Lemmas.lemma_div_lt (v u0) 52 4;
+  Math.Lemmas.cancel_mul_mod (v u0) (pow2 4);
+  logor_disjoint tx (u0 <<. 4ul) 4;
+  assert (v u0' == v tx + v u0 * pow2 4);
+  assert (v u0' < pow2 56)
+
+
+val lemma_mod_add_last (c12 t4':uint64) : Lemma
+  (requires v c12 < pow2 42 /\ v t4' < pow2 48)
+  (ensures (let r4 = c12 +. t4' in
+    v r4 = v c12 + v t4' /\ felem_fits_last1 r4 2))
+
+let lemma_mod_add_last c12 t4' =
+  let r4 = c12 +. t4' in
+  assert (v c12 + v t4' < pow2 42 + pow2 48);
+  Math.Lemmas.pow2_lt_compat 48 42;
+  Math.Lemmas.pow2_double_sum 48;
+  assert (v c12 + v t4' < pow2 49);
+  Math.Lemmas.pow2_lt_compat 64 49;
+  Math.Lemmas.small_mod (v c12 + v t4') (pow2 64);
+  assert (v r4 = v c12 + v t4')
+
+
+#set-options "--z3rlimit 150"
+
+val fmul5_lemma: a:felem5 -> b:felem5 -> Lemma
+  (requires
+    felem_fits5 a (8,8,8,8,8) /\
+    felem_fits5 b (8,8,8,8,8))
+  (ensures (let res = fmul5 a b in
+    as_nat5 res % S.prime == as_nat5 a * as_nat5 b % S.prime  /\
+    felem_fits5 res (1,1,1,1,2)))
+
+let fmul5_lemma a b =
+  let (a0,a1,a2,a3,a4) = a in
+  let (b0,b1,b2,b3,b4) = b in
+
+  let r = u64 0x1000003D10 in
+
+  let d0 = mul64_wide a0 b3
+       +. mul64_wide a1 b2
+       +. mul64_wide a2 b1
+       +. mul64_wide a3 b0 in
+  lemma_four_mul64_wide a0 a1 a2 a3 b0 b1 b2 b3;
+  assert (v d0 = v a0 * v b3 + v a1 * v b2 + v a2 * v b1 + v a3 * v b0);
+  assert (v d0 <= 256 * (max52 * max52));
+
+  let c0 = mul64_wide a4 b4 in
+  lemma_bound_mul64_wide 8 8 max48 max48 a4 b4;
+  assert (v c0 = v a4 * v b4);
+  assert (v c0 <= 64 * (max48 * max48));
+
+  let d1 = d0 +. mul64_wide r (to_u64 c0) in let c1 = to_u64 (c0 >>. 64ul) in
+  lemma_bound_add_mul64_wide_r 256 d0 c0;
+  assert (v d1 = v d0 + v r * (v c0 % pow2 64));
+  assert (v d1 <= 257 * (max52 * max52));
+  lemma_bound_rsh64_to c0;
+  assert (v c1 = v c0 / pow2 64);
+  lemma_bound_c0 c0;
+  assert (v c1 <= pow2 38);
+
+  let t3 = to_u64 d1 &. mask52 in let d2 = d1 >>. 52ul in
+  lemma_bound_mask52_rsh52 257 d1;
+  assert (v t3 = v d1 % pow2 52);
+  assert (felem_fits1 t3 1);
+  assert (v d2 = v d1 / pow2 52);
+  assert (v d2 <= 257 * max52);
+
+  let d3 = d2
+       +. mul64_wide a0 b4
+       +. mul64_wide a1 b3
+       +. mul64_wide a2 b2
+       +. mul64_wide a3 b1
+       +. mul64_wide a4 b0 in
+  lemma_add_five_mul64_wide 257 d2 a0 a1 a2 a3 a4 b0 b1 b2 b3 b4;
+  assert (v d3 == v d2 + v a0 * v b4 + v a1 * v b3 + v a2 * v b2 + v a3 * v b1 + v a4 * v b0);
+  assert (v d3 <= 201 * (max52 * max52));
+
+  let d4 = d3 +. mul64_wide (r <<. 12ul) c1 in
+  lemma_bound_add_mul64_wide_r_lsh12 201 d3 c1;
+  assert (v d4 == v d3 + v r * pow2 12 * v c1);
+  assert (v d4 <= 202 * (max52 * max52));
+
+  let t4 = to_u64 d4 &. mask52 in let d5 = d4 >>. 52ul in
+  lemma_bound_mask52_rsh52 202 d4;
+  assert (v t4 = v d4 % pow2 52);
+  assert (felem_fits1 t4 1);
+  assert (v d5 = v d4 / pow2 52);
+  assert (v d5 <= 202 * max52);
+
+  let tx = t4 >>. 48ul in let t4' = t4 &. mask48 in
+  lemma_bound_mask48_rsh48 t4;
+  assert (v tx = v t4 / pow2 48);
+  assert (v tx < pow2 4);
+  assert (v t4' = v t4 % pow2 48);
+  assert (felem_fits_last1 t4' 1);
+
+  let c2 = mul64_wide a0 b0 in
+  lemma_bound_mul64_wide 8 8 max52 max52 a0 b0;
+  assert (v c2 = v a0 * v b0);
+  assert (v c2 <= 64 * (max52 * max52));
+
+  let d6 = d5
+       +. mul64_wide a1 b4
+       +. mul64_wide a2 b3
+       +. mul64_wide a3 b2
+       +. mul64_wide a4 b1 in
+  lemma_add_four_mul64_wide 202 d5 a1 a2 a3 a4 b1 b2 b3 b4;
+  assert (v d6 == v d5 + v a1 * v b4 + v a2 * v b3 + v a3 * v b2 + v a4 * v b1);
+  assert (v d6 <= 201 * (max52 * max52));
+
+  let u0 = to_u64 d6 &. mask52 in let d7 = d6 >>. 52ul in
+  lemma_bound_mask52_rsh52 201 d6;
+  assert (v u0 = v d6 % pow2 52);
+  assert (felem_fits1 u0 1);
+  assert (v d7 = v d6 / pow2 52);
+  assert (v d7 <= 201 * max52);
+
+  let u0' = tx |. (u0 <<. 4ul) in
+  lemma_tx_logor_u0_lsh4 tx u0;
+  assert (v u0' == v tx + v u0 * pow2 4);
+  assert (v u0' < pow2 56);
+
+  let c3 = c2 +. mul64_wide u0' (r >>. 4ul) in
+  lemma_bound_add_mul64_wide_r_rsh4 64 c2 u0';
+  assert (v c3 = v c2 + v u0' * (v r / pow2 4));
+  assert (v c3 <= 65 * (max52 * max52));
+
+  let r0 = to_u64 c3 &. mask52 in let c4 = c3 >>. 52ul in
+  lemma_bound_mask52_rsh52 65 c3;
+  assert (v r0 = v c3 % pow2 52);
+  assert (felem_fits1 r0 1);
+  assert (v c4 = v c3 / pow2 52);
+  assert (v c4 <= 65 * max52);
+
+  let c5 = c4
+       +. mul64_wide a0 b1
+       +. mul64_wide a1 b0 in
+  lemma_add_two_mul64_wide52 65 c4 a0 a1 b0 b1;
+  assert (v c5 = v c4 + v a0 * v b1 + v a1 * v b0);
+  assert (v c5 <= 129 * (max52 * max52));
+
+  let d8 = d7
+       +. mul64_wide a2 b4
+       +. mul64_wide a3 b3
+       +. mul64_wide a4 b2 in
+  lemma_add_three_mul64_wide 320 d7 a2 a3 a4 b2 b3 b4;
+  assert (v d8 = v d7 + v a2 * v b4 + v a3 * v b3 + v a4 * v b2);
+  assert (v d8 <= 129 * (max52 * max52));
+
+  let c6 = c5 +. mul64_wide (to_u64 d8 &. mask52) r in let d9 = d8 >>. 52ul in
+  lemma_bound_add_mul64_wide_r_mask52 129 d8 c5;
+  assert (v d9 = v d8 / pow2 52);
+  assert (v d9 <= 129 * max52);
+  assert (v c6 = v c5 + v d8 % pow2 52 * v r);
+  assert (v c6 <= 130 * (max52 * max52));
+
+  let r1 = to_u64 c6 &. mask52 in let c7 = c6 >>. 52ul in
+  lemma_bound_mask52_rsh52 130 c6;
+  assert (v r1 = v c6 % pow2 52);
+  assert (felem_fits1 r1 1);
+  assert (v c7 = v c6 / pow2 52);
+  assert (v c7 <= 130 * max52);
+
+  let c8 = c7
+       +. mul64_wide a0 b2
+       +. mul64_wide a1 b1
+       +. mul64_wide a2 b0 in
+  lemma_add_three_mul64_wide52 130 c7 a0 a1 a2 b0 b1 b2;
+  assert (v c8 == v c7 + v a0 * v b2 + v a1 * v b1 + v a2 * v b0);
+  assert (v c8 <= 193 * (max52 * max52));
+
+  let d10 = d9
+       +. mul64_wide a3 b4
+       +. mul64_wide a4 b3 in
+  lemma_add_two_mul64_wide 129 d9 a3 a4 b3 b4;
+  assert (v d10 == v d9 + v a3 * v b4 + v a4 * v b3);
+  assert (v d10 <= 9 * (max52 * max52));
+
+  let c9 = c8 +. mul64_wide r (to_u64 d10) in let d11 = to_u64 (d10 >>. 64ul) in
+  lemma_bound_add_mul64_wide_r 193 c8 d10;
+  assert (v c9 = v c8 + v r * (v d10 % pow2 64));
+  assert (v c9 <= 194 * (max52 * max52));
+  lemma_bound_rsh64_to d10;
+  assert (v d11 = v d10 / pow2 64);
+  lemma_bound_d10 d10;
+  assert (v d11 < pow2 44);
+
+  let r2 = to_u64 c9 &. mask52 in let c10 = c9 >>. 52ul in
+  lemma_bound_mask52_rsh52 194 c9;
+  assert (v r2 = v c9 % pow2 52);
+  assert (felem_fits1 r2 1);
+  assert (v c10 = v c9 / pow2 52);
+  assert (v c10 <= 194 * max52);
+
+  let c11 = c10 +. mul64_wide (r <<. 12ul) d11 +. to_u128 t3 in
+  lemma_bound_add_mul64_wide_r_lsh12_add 194 c10 d11 t3;
+  assert (v c11 = v c10 + v r * pow2 12 * v d11 + v t3);
+  assert (v c11 < pow2 94);
+
+  let r3 = to_u64 c11 &. mask52 in let c12 = to_u64 (c11 >>. 52ul) in
+  lemma_bound_mask52_rsh52_sp c11;
+  assert (v r3 = v c11 % pow2 52);
+  assert (felem_fits1 r3 1);
+  assert (v c12 = v c11 / pow2 52);
+  assert (v c12 < pow2 42);
+
+  let r4 = c12 +. t4' in
+  lemma_mod_add_last c12 t4';
+  assert (v r4 = v c12 + v t4');
+  assert (felem_fits_last1 r4 2);
+
+  let res = (r0,r1,r2,r3,r4) in
+  assert (res == fmul5 a b);
+  assert (felem_fits5 res (1,1,1,1,2));
+
+  L4.lemma_fmul_simplify (v r0) (v r1) (v r2) (v r3) (v r4)
+    (v c3) (v c6) (v c9) (v c11) (v d4) (v d8) (v d10) (v d11)
+    (v t3) (v a0) (v a1) (v a2) (v a3) (v a4) (v b0) (v b1) (v b2) (v b3) (v b4)
